 
\chapter*{Integrales}

\begin{minipage}[c]{0.5\textwidth}
\begin{align*}
& \int x^n\,\,dx = \frac{x^{n+1}}{n+1} , \,\,\,n \neq -1\\
& \int \frac{dx}{x} = \ln |x|\\
& \int \frac{dx}{a+bx} = \frac{\ln (a+bx)}{b}\\
& \int \frac{x}{a+bx} = \frac{x}{b} - \frac{a}{b^2}\ln(a+bx)\\
& \int \frac{dx}{x(a+bx)} = -\frac{1}{a}\ln\left( \frac{x+a}{x} \right)\\
& \int \frac{dx}{(a+bx)^2} = -\frac{1}{b(a+bx)}\\
& \int \frac{dx}{a^2+x^2} = \frac{1}{a}\tan^{-1} \left( \frac{x}{a} \right)\\
& \int \frac{dx}{a^2-x^2} = \frac{1}{a}\tanh^{-1} \left( \frac{x}{a} \right)\\
& \int \frac{dx}{x^2-a^2} = -\frac{1}{a}\tanh^{-1} \left( \frac{x}{a} \right)\\
& \int \frac{x}{x^2 \pm a^2}\,\,dx = \pm \frac{1}{2} \ln (a^2\pm x^2)\\
& \int \frac{dx}{\sqrt{a^2 - x^2}} =  \sen^{-1} \left( \frac{x}{a} \right),\,\,\,\,a^2-x^2 >0\\
& \int \frac{dx}{\sqrt{x^2 \pm a^2}} =  \ln \left( x+\sqrt{x^2 \pm a^2} \right)\\
& \int \frac{x}{\sqrt{a^2 - x^2}}\,\,dx = -\sqrt{a^2-x^2}\\
& \int \frac{x}{\sqrt{x^2 \pm a^2}}\,\,dx = \sqrt{x^2 \pm a^2}\\
& \int \sqrt{a^2 - x^2}\,\,dx = \frac{1}{2}\left[ x\sqrt{a^2-x^2} + a^2\sen^{-1} \left( \frac{x}{a} \right) \right] \\
& \int x\sqrt{a^2 - x^2}\,\,dx =  -\frac{1}{3}(a^2-x^2)^{3/2}\\
& \int \sqrt{x^2 \pm a^2}\,\,dx =  \frac{1}{3} \left[ x\sqrt{x^2 \pm a^2} \pm a^2\ln \left(x+\sqrt{x^2 \pm a^2} \right) \right] \\
& \int x\sqrt{x^2 \pm a^2}\,\,dx =  \frac{1}{3}(a^2\pm a^2)^{3/2}\\
& \int e^{ax}\,\,dx = \frac{1}{a}e^{ax}
\end{align*}
\end{minipage}
\begin{minipage}[c]{0.5\textwidth}
\begin{align*}
& \int \ln (ax)\,\,dx = x\ln (ax) -x\\
& \int xe^{ax}\,\,dx = \frac{e^{ax}}{a^2}(ax-1)\\
& \int \frac{dx}{a+bx^{cx}} = \frac{x}{a} - \frac{1}{ac}\ln \left( a+bx^{cx} \right) \\
& \int \sen (ax)\,\,dx = -\frac{1}{a}\cos(ax)\\
& \int \cos (ax)\,\,dx = \frac{1}{a}\sen(ax)\\
& \int \tan (ax)\,\,dx = \frac{1}{a}\ln [\sec (ax)]\\
& \int \cot (ax)\,\,dx = \frac{1}{a}\ln [\sen (ax)]\\
& \int \sec (ax)\,\,dx = \frac{1}{a}\ln [\sec (ax) + \tan(ax)]  \\
& \int \csc (ax)\,\,dx = \frac{1}{a}\ln [\csc (ax) - \cot(ax)]\\
& \int \sen^2 (ax)\,\,dx = \frac{x}{2} - \frac{\sen (2ax)}{4a}\\
& \int \cos^2 (ax)\,\,dx = \frac{x}{2} + \frac{\sen (2ax)}{4a}\\
& \int \frac{dx}{\sen^2(ax)} = -\frac{1}{a}\cot (ax)\\
& \int \frac{dx}{\cos^2(ax)} = \frac{1}{a}\tan (ax)\\
& \int \tan^2 (ax)\,\,dx = \frac{1}{a}\tan(ax) -x \\
& \int \cot^2 (ax)\,\,dx = -\frac{1}{a}\cot(ax)  -x \\
& \int \sen^{-1} (ax)\,\,dx = x\sen^{-1}(ax) + \frac{\sqrt{1-a^2x^2}}{a} \\
& \int \cos^{-1} (ax)\,\,dx = x\cos^{-1}(ax) - \frac{\sqrt{1-a^2x^2}}{a} \\
& \int \frac{dx}{(x^2+a^2)^{3/2}} = -\frac{x}{a^2\sqrt{x^2+a^2}}  \\
& \int \frac{x}{(x^2+a^2)^{3/2}}\,\,dx = -\frac{1}{\sqrt{x^2+a^2}} 
\end{align*}
\end{minipage}

\begin{minipage}[c]{0.5\textwidth}
\begin{align*}
& \int x\sen (ax)\,\,dx = \frac{1}{a^2} \left( \sin(ax) -ax\cos(ax) \right)\\
& \int x\cos (ax)\,\,dx = \frac{1}{a^2} \left( \cos(ax) +ax\sen(ax) \right)\\
& \int x^2\sen (ax)dx = \frac{1}{a^3} \left(-a^2x^2 \cos(ax) +2\cos(ax) + 2ax\sen(ax) \right)\\
& \int x^2\cos (ax)dx = \frac{1}{a^3} \left(-a^2x^2 \sen(ax) -2\sen(ax) + 2ax\cos(ax) \right)\\
& \int \sqrt{x^2\pm a^2}dx =  \frac{x}{2}\sqrt{x^2 \pm a^2} \pm \frac{a^2}{2}\ln \left( x+\sqrt{x^2\pm a^2} \right)
\end{align*}
\end{minipage}
\begin{minipage}[c]{0.5\textwidth}
\begin{align*}
& \int \frac{x}{\sqrt{x^2 \pm a^2}}\,\,dx = \sqrt{x^2\pm a^2}\\
& \int \frac{x}{\sqrt{a^2-x^2}}\,\,dx = -\sqrt{a^2-x^2}\\
& \int x\sqrt{a^2-x^2}\,\,dx = -\frac{x}{3} \left( a^2-x^2 \right)^{3/2} \\
& \int \sqrt{a^2-x^2}dx = \frac{1}{2} \left[ x\sqrt{a^2-x^2} -a^2\sen^{-1}\left(\frac{x}{a} \right) \right] \\
& \int x\sqrt{x^2\pm a^2}dx = \frac{x}{3} \left( x^2-a^2 \right)^{3/2}
\end{align*}
\end{minipage}
\subsection*{Integral de probabilidad de Gauss}
\begin{align*}
& I_0 = \int_0^\infty e^{-ax^2}\,\, dx = \frac{1}{2}\sqrt{\frac{\pi}{a}}\\
& I_1 = \int_0^\infty xe^{-ax^2}\,\, dx = \frac{1}{2a}\\
& I_2 = \int_0^\infty x^2e^{-ax^2}\,\, dx = -\frac{dI_0}{da}= \frac{1}{4}\sqrt{\frac{\pi}{a^3}}\\
& I_3 = \int_0^\infty x^3e^{-ax^2}\,\, dx =-\frac{dI_1}{da}= \frac{1}{2a} \\
& I_4 = \int_0^\infty x^4e^{-ax^2}\,\, dx = \frac{d^2I_0}{da^2}= \frac{3}{8}\sqrt{\frac{\pi}{a^5}}\\
& I_5 = \int_0^\infty x^5e^{-ax^2}\,\, dx = \frac{d^2I_1}{da^2}= \frac{1}{a^3}\\
& \cdot\\
& \cdot\\
& I_{2n} = (-1)^n\frac{d^n}{da^n}I_0\\
& I_{2n+1} = (-1)^n\frac{d^n}{da^n}I_1
\end{align*}